Attempt at compatibility Lemma for non-recursive let-bindings

src/Language/PlutusIR/Semantics/SemanticEquivalence/FundamentalProperty.v
@@ -7,21 +7,23 @@ Require Import PlutusCert.Language.PlutusIR.Semantics.TypeSafety.SubstitutionPre
 Require Import PlutusCert.Language.PlutusIR.Semantics.SemanticEquivalence.CompatibilityLemmas.
 Require Import PlutusCert.Language.PlutusIR.Semantics.SemanticEquivalence.LogicalRelation.RelationalModel.
 Require Import PlutusCert.Language.PlutusIR.Semantics.SemanticEquivalence.Monotonicity.
-
+Require Import PlutusCert.Util.
 
 (** ** The [R] Lemma *)
 
 
-Definition P_has_type Gamma e T := 
-  LR_logically_approximate (fst Gamma) (snd Gamma) e e T.
+Definition P_has_type ctx e T := 
+  LR_logically_approximate (fst ctx) (snd ctx) e e T.
 
-Definition P_constructor_well_formed Gamma c := Gamma |-ok_c c.
+Definition P_constructor_well_formed ctx c := ctx |-ok_c c.
 
-Definition P_bindings_well_formed_nonrec Gamma bs1 := Gamma |-oks_nr bs1.
+Definition P_bindings_well_formed_nonrec ctx bs := 
+  LR_logically_approximate_bindings_nonrec (fst ctx) (snd ctx) bs bs.
 
-Definition P_bindings_well_formed_rec Gamma bs1 := Gamma |-oks_r bs1.
+Definition P_bindings_well_formed_rec ctx bs1 := ctx |-oks_r bs1.
 
-Definition P_binding_well_formed Gamma b1 := Gamma |-ok b1.
+Definition P_binding_well_formed ctx b := 
+  LR_logically_approximate_binding (fst ctx) (snd ctx) b b.
 
 Axiom skip : forall P, P.
 
@@ -35,9 +37,11 @@ Axiom skip : forall P, P.
       msubst e2 t2 t2' ->
       R T t1' t2'.*)
 
-Lemma msubst_R : forall Gamma e T,
-    Gamma |-+ e : T ->
-    P_has_type Gamma e T.
+
+
+Lemma msubst_R : forall ctx e T,
+    ctx |-+ e : T ->
+    P_has_type ctx e T.
 Proof.
   apply has_type__ind with 
     (P := P_has_type)
@@ -48,16 +52,13 @@ Proof.
 
   all : unfold P_has_type; intros; subst.
   all : eauto with DSP_compatibility_lemmas.
-  - intros. unfold P_has_type. intros. subst.
-    apply skip.
-  - intros. unfold P_has_type. intros. subst.
-    apply skip.
+  - apply skip.
   - unfold P_constructor_well_formed. eauto with typing.
-  - unfold P_bindings_well_formed_nonrec. eauto with typing.
-  - unfold P_bindings_well_formed_nonrec. eauto with typing.
+  - unfold P_bindings_well_formed_nonrec. constructor. 
+  - unfold P_bindings_well_formed_nonrec. econstructor; eauto with DSP_compatibility_lemmas.
   - unfold P_bindings_well_formed_rec. eauto with typing.
   - unfold P_bindings_well_formed_rec. eauto with typing.
-  - unfold P_binding_well_formed. eauto with typing.
-  - unfold P_binding_well_formed. eauto with typing.
-  - unfold P_binding_well_formed. eauto with typing. 
+  - apply skip. (* TODO *)
+  - apply skip. (* TODO *)
+  - apply skip. (* TODO *)
 Qed.
