src/Language/PlutusIR/Semantics/SemanticEquivalence/CompatibilityLemmas.v
@@ -4,6 +4,7 @@ Require Export PlutusCert.Language.PlutusIR.Semantics.SemanticEquivalence.Compat
 Require Export PlutusCert.Language.PlutusIR.Semantics.SemanticEquivalence.CompatibilityLemmas.Error.
 Require Export PlutusCert.Language.PlutusIR.Semantics.SemanticEquivalence.CompatibilityLemmas.IWrap.
 Require Export PlutusCert.Language.PlutusIR.Semantics.SemanticEquivalence.CompatibilityLemmas.LamAbs.
+Require Export PlutusCert.Language.PlutusIR.Semantics.SemanticEquivalence.CompatibilityLemmas.LetNonRec.
 Require Export PlutusCert.Language.PlutusIR.Semantics.SemanticEquivalence.CompatibilityLemmas.Unwrap.
 Require Export PlutusCert.Language.PlutusIR.Semantics.SemanticEquivalence.CompatibilityLemmas.TyAbs.
 Require Export PlutusCert.Language.PlutusIR.Semantics.SemanticEquivalence.CompatibilityLemmas.TyInst.
@@ -18,7 +19,15 @@ Create HintDb DSP_compatibility_lemmas.
   compatibility_Error
   compatibility_IWrap
   compatibility_LamAbs
+  compatibility_LetNonRec
   compatibility_TyAbs
   compatibility_TyInst
   compatibility_Unwrap
   compatibility_Var : DSP_compatibility_lemmas.
+
+
+Lemma distr_projection_application : forall {A B C D: Type} (f : A * B -> C * D) (p : A * B),
+    (fst (f p), snd (f p)) = f (fst p, snd p).
+Proof. destruct p. simpl. destruct f. simpl. reflexivity. Qed.
+
+#[export] Hint Resolve distr_projection_application : DSP_compatibility_lemmas.
