src/Language/PlutusIR/Semantics/SemanticEquivalence/CompatibilityLemmas/LetNonRec.v
@@ -1,0 +1,80 @@
+Require Import PlutusCert.Language.PlutusIR.
+Import NamedTerm.
+Require Import PlutusCert.Language.PlutusIR.Semantics.Dynamic.
+Require Import PlutusCert.Language.PlutusIR.Semantics.Static.
+Require Import PlutusCert.Language.PlutusIR.Semantics.SemanticEquivalence.LogicalRelation.RelationalModel.
+Require Import PlutusCert.Language.PlutusIR.Semantics.SemanticEquivalence.Monotonicity.
+
+Require Import Arith.
+
+Lemma compatibility_LetNonRec : forall Delta Gamma bs t bs' t' T,
+    forall Delta' Gamma',
+      (Delta', Gamma') = append (flatten (List.map binds bs)) (Delta, Gamma) ->
+      LR_logically_approximate Delta' Gamma' t t' T ->
+      LR_logically_approximate_bindings_nonrec Delta Gamma bs bs' ->
+      LR_logically_approximate Delta Gamma (Let NonRec bs t) (Let NonRec bs' t') T.
+Proof.
+  intros Delta Gamma bs t bs' t' T Delta' Gamma' Hbinds IH_LR__t IH_LR__bs.
+  unfold LR_logically_approximate.
+
+  split. {
+    eapply T_Let.
+    - apply Hbinds.
+    - eapply LR_la_bnr__oks in IH_LR__bs. 
+      apply IH_LR__bs. 
+    - apply IH_LR__t.  
+  }
+
+  split. {
+    eapply T_Let.
+    - eapply LR_la_bnr__oks in IH_LR__bs.
+      destruct IH_LR__bs as [_ [_ Heq]].
+      rewrite <- Heq.
+      apply Hbinds.
+    - eapply LR_la_bnr__oks in IH_LR__bs.
+      apply IH_LR__bs.
+    - apply IH_LR__t.
+  }
+
+  intros k rho env env' ct ck HeqDelta HeqGamma [H_RD H_RG].
+  subst.
+
+  (*
+  intros e_sa e'_sa e_s e'_s.
+  intros HmsA__e_sa HmsA__e'_sa Hms__e_s Hms__e'_s.
+
+  destruct (msubstA_LamAbs _ _ _ _ _ HmsA__e_sa) as [eb_sa [HmsA__eb_sa Heq]].
+  destruct (msubstA_LamAbs _ _ _ _ _ HmsA__e'_sa) as [eb'_sa [HmsA__eb'_sa Heq']].
+  subst.
+  destruct (msubst_LamAbs _ _ _ _ _ Hms__e_s) as [eb_s [Hms__eb_s Heq]].
+  destruct (msubst_LamAbs _ _ _ _ _ Hms__e'_s) as [eb'_s [Hms__eb'_s Heq']].
+  subst.
+
+  autorewrite with RC.
+  split. {
+    replace emptyContext with (@empty Kind, mupd (msyn1 rho) empty).
+    - eapply msubst_preserves_typing_1; eauto.
+      eapply msubstA_preserves_typing_1; eauto.
+      destruct IH_LR.
+      eapply T_LamAbs; eauto.
+    - rewrite mupd_empty; eauto.
+  }
+  split. {
+    replace emptyContext with (@empty Kind, mupd (msyn2 rho) empty).
+    - eapply msubst_preserves_typing_2; eauto.
+      eapply msubstA_preserves_typing_2; eauto.
+      destruct IH_LR. destruct H0.
+      eapply T_LamAbs; eauto.
+    - rewrite mupd_empty; eauto.
+  }
+
+  intros j Hlt__j e_f Hev__e_f.
+  inversion Hev__e_f. subst.
+  exists (LamAbs x (msubstT (msyn2 rho) T1) eb'_s).
+  exists 0.
+  split. {
+    eapply eval_value. apply V_LamAbs.
+  }
+  intros.
+  *)
+Admitted.
